finished some proofs

lambda.v
@@ -87,6 +87,13 @@ Proof.
   reflexivity.
 Qed.
 
+Example sanity2:
+  (var 0 ⋅ var 1 ⋅ var 2) =
+  ((var 0 ⋅ var 1) ⋅ var 2).
+Proof.
+  reflexivity.
+Qed.
+
 Example omega_step:
   step Omega Omega.
 Proof.
@@ -99,7 +106,7 @@ Qed.
 Definition equivalent e1 e2 := 
   exists e3, steps e1 e3 /\ steps e2 e3.
 
-Notation "e1 ≡ e2" := (equivalent e1 e2) (at level 0).
+Notation "e1 ≡ e2" := (equivalent e1 e2) (at level 70).
 
 
 
@@ -205,6 +212,11 @@ B0 := λ x y. x
 B1 := λ x y. y
 *)
 
+Definition nil := λ, λ, var 1.
+Definition cons v vs := λ, λ, var 1 ⋅ v ⋅ vs.
+Definition B0 := λ, λ, var 0.
+Definition B1 := λ, λ, var 1.
+
 (*
 
 F = Y (λ e c s. s (λ a. a F0 F1))
@@ -226,6 +238,320 @@ F1 C F (enc A ++ enc B ++ ys)
 *)
 
 Definition F0 C :=
-  λ, var 0 ⋅ (λ, C ⋅ (var 1 ⋅ lam_K ⋅ lam_S)).
+  λ, var 0 ⋅ (λ, C ⋅ (var 0 ⋅ lam_K ⋅ lam_S)).
 Definition F1 C F :=
   F ⋅ (λ, F ⋅ (λ, C ⋅ (var 1 ⋅ var 0))).
+
+Definition F' := 
+  (* λ f c s. s *)
+  (λ, λ, λ, var 0 ⋅ 
+    (* λ a. a F0 F1 *)
+    (* F0 C, F1 C F *)
+    (λ, var 0 ⋅ (F0 (var 2) ⋅ F1 (var 2) (var 3)))).
+Definition F := lam_Y ⋅ F'.
+
+
+(* Ltac clear_lift_subst :=
+  let rec f :=
+    repeat (setoid_rewrite closed_lift;[|resolve_closed]);
+    repeat (setoid_rewrite closed_subst;[|resolve_closed])
+  with resolve_closed :=
+    clear_lift_subst;
+    cbn;firstorder;try lia;now eauto
+  in f. *)
+
+Hint Resolve closed_inc : core.
+
+Ltac resolve_closed :=
+  cbn;firstorder;lia;now auto.
+
+(* Ltac resolve_closed :=
+  clear_lift_subst;
+  cbn;firstorder;try lia;now eauto
+  with
+Ltac clear_lift_subst :=
+  repeat (setoid_rewrite closed_lift;[|resolve_closed]);
+  repeat (setoid_rewrite closed_subst;[|resolve_closed]). *)
+  (* repeat (
+    setoid_rewrite closed_lift;[|
+    firstorder;try lia;now eauto]);
+  repeat setoid_rewrite closed_subst;
+  (repeat apply closed_inc;try easy). *)
+
+Ltac clear_lift_subst :=
+  repeat setoid_rewrite closed_lift;
+  repeat setoid_rewrite closed_subst;
+  try resolve_closed.
+
+Lemma steps_beta e1 e2:
+  steps (app (lam e1) e2) (subst0 e2 e1).
+Proof.
+  eapply steps_step; [apply step_beta|];cbn.
+  apply steps_refl.
+Qed.
+
+(* contextual semantics lift *)
+Lemma steps_lam e1 e2:
+  steps e1 e2 -> steps (lam e1) (lam e2).
+Proof.
+  induction 1.
+  - constructor.
+  - eapply steps_step.
+    2: now apply IHsteps.
+    now apply step_lam.
+Qed.
+
+Lemma steps_app_left e1 e2 e:
+  steps e1 e2 -> steps (app e1 e) (app e2 e).
+Proof.
+  induction 1.
+  - constructor.
+  - eapply steps_step.
+    2: now apply IHsteps.
+    now apply step_app_left.
+Qed.
+
+Lemma steps_app_right e1 e2 e:
+  steps e1 e2 -> steps (app e e1) (app e e2).
+Proof.
+  induction 1.
+  - constructor.
+  - eapply steps_step.
+    2: now apply IHsteps.
+    now apply step_app_right.
+Qed.
+
+Lemma steps_trans e1 e2 e3:
+  steps e1 e2 -> steps e2 e3 -> steps e1 e3.
+Proof.
+  intros H1 H2.
+  induction H1.
+  - easy.
+  - eapply steps_step.
+    2: now apply IHsteps.
+    easy.
+Qed.
+
+Definition F0_spec C a xs :=
+  (F0 C) ⋅ (cons a xs) ≡ λ, C ⋅ (a ⋅ lam_K ⋅ lam_S) ⋅ xs.
+
+Lemma F0_spec_proof C a xs:
+  closed0 C -> closed0 a -> closed0 xs ->
+  F0_spec C a xs.
+Proof.
+  unfold F0_spec.
+  intros HC_C HC_a HC_xs.
+  unfold cons, F0.
+  (* remember lam_K as K.
+  remember lam_S as S. *)
+  eexists;split. 
+  2: apply steps_refl.
+  - eapply steps_trans.
+    apply steps_beta.
+    cbn;clear_lift_subst.
+
+    eapply steps_trans.
+    apply steps_beta.
+    cbn;clear_lift_subst.
+
+    eapply steps_trans.
+    apply steps_lam, steps_app_left, steps_beta.
+    cbn;clear_lift_subst.
+
+    fold lam_K lam_S.
+    apply steps_refl.
+Qed.
+
+Inductive SK : Type :=
+  | S : SK
+  | K : SK
+  | SK_app : SK -> SK -> SK.
+
+Fixpoint encode (s : SK) : list bool :=
+  match s with
+  | K => [false;false]
+  | S => [false;true]
+  | SK_app s1 s2 => true::encode s1 ++ encode s2
+  end.
+
+Fixpoint encode_list (l : list SK) : list bool :=
+  match l with
+  | [] => []
+  | x::xs => encode x ++ encode_list xs
+  end.
+
+Fixpoint to_lam (s : SK) : lambda :=
+  match s with
+  | K => lam_K
+  | S => lam_S
+  | SK_app s1 s2 => app (to_lam s1) (to_lam s2)
+  end.
+
+Fixpoint embed_list (l : list bool) : lambda :=
+  match l with
+  | [] => nil
+  | x::xs => cons (if x then B1 else B0) (embed_list xs)
+  end.
+
+Definition F_spec C (x:SK) (xs:list SK) :=
+  (* F ⋅ C ⋅ (embed_list (encode_list (x::xs))) ≡ C ⋅ (to_lam x) ⋅ (embed_list(encode_list xs)). *)
+  F ⋅ C ⋅ (embed_list (encode x ++ encode_list xs)) ≡ C ⋅ (to_lam x) ⋅ (embed_list(encode_list xs)).
+
+Lemma equiv_trans e1 e2 e3:
+  e1 ≡ e2 -> e2 ≡ e3 -> e1 ≡ e3.
+Proof.
+  intros (e12&H1_2&H2_1).
+  intros (e23&H2_3&H3_2).
+  (* confluence at e2 -> e12, e23 *)
+Admitted.
+
+Definition F1_spec C A B xs :=
+  (F1 C F) ⋅ 
+  embed_list (encode A ++ encode B ++ encode_list xs) ≡ 
+  C ⋅ (to_lam A ⋅ to_lam B) ⋅ (embed_list (encode_list xs)).
+
+(* Lemma closed_F : closed0 F.
+Proof.
+  unfold F; firstorder;cbn;lia.
+Qed.
+
+Lemma closed_F' : closed0 F'.
+Proof.
+  firstorder;cbn;lia.
+Qed.
+
+Lemma closed_Y : closed0 lam_Y.
+Proof.
+  firstorder;cbn;lia.
+Qed.*)
+
+Lemma closed_SK x: closed0 (to_lam x).
+Proof.
+  induction x;cbn;try easy;lia.
+Qed. 
+
+Hint Resolve closed_SK.
+
+Lemma F1_spec_proof C A B xs:
+  (forall C x xs, closed0 C -> F_spec C x xs) ->
+  closed0 C -> 
+  F1_spec C A B xs.
+Proof.
+  intros F_spec_proof HC_C.
+  unfold F1_spec, F1.
+  remember (to_lam A) as Al.
+  remember (to_lam B) as Bl.
+  eapply equiv_trans.
+  {
+    remember (λ, F ⋅ (λ, C ⋅ (var 1 ⋅ var 0))) as Cont.
+    pose proof (F_spec_proof Cont A (B::xs)).
+    unfold F_spec in H; cbn in H.
+    subst.
+    apply H.
+    resolve_closed.
+  }
+  eapply equiv_trans.
+  {
+    eexists;split;[|apply steps_refl].
+    apply steps_app_left.
+    apply steps_beta.
+  }
+  cbn -[F].  clear_lift_subst.
+  (* cbn -[F].  clear_lift_subst;try now first [apply closed_F|apply closed_SK]. *)
+  eapply equiv_trans.
+  {
+    apply F_spec_proof.
+    clear_lift_subst.
+    (* firstorder;cbn;try lia. *)
+    (* all: apply closed_inc; 
+        now first [assumption|apply closed_SK]. *)
+  }
+  eexists;split;[|apply steps_refl].
+  apply steps_app_left.
+  eapply steps_step.
+  1: apply step_beta.
+  cbn;clear_lift_subst.
+  (* all: try apply closed_SK. *)
+  now subst; apply steps_refl.
+Defined.
+
+Lemma equiv_app_left e1 e2 e3:
+  e1 ≡ e2 -> e1 ⋅ e3 ≡ e2 ⋅ e3.
+Proof.
+  intros (e12&H1_2&H2_1).
+  eexists;split.
+  all: apply steps_app_left;eassumption.
+Qed.
+
+(* Hint Resolve closed_inc : core. *)
+(* Hint Resolve closed_F : core.
+Hint Resolve closed_Y : core.
+Hint Resolve closed_F' : core. *)
+
+Lemma F_spec_proof C ys:
+  closed0 C -> 
+  match ys with
+  | [] => F ⋅ C ⋅ nil ≡ λ, var 0
+  | x::xs => F_spec C x xs
+  end.
+Proof.
+  induction ys as [|x xs IH].
+  - intros HC_C.
+    unfold F.
+    eapply equiv_trans.
+    {
+      do 2 apply equiv_app_left.
+      apply fixpoint.
+      resolve_closed.
+    }
+    eexists;split;[|apply steps_refl].
+
+    eapply steps_trans.
+    do 2 apply steps_app_left.
+    apply steps_beta.
+    cbn -[lam_Y F0 F']; clear_lift_subst.
+
+    eapply steps_trans.
+    apply steps_app_left.
+    apply steps_beta.
+    cbn -[lam_Y F0 F']; clear_lift_subst.
+
+    eapply steps_trans.
+    apply steps_beta.
+    cbn -[lam_Y F0 F']; clear_lift_subst.
+
+    eapply steps_trans.
+    apply steps_beta.
+    cbn -[lam_Y F0 F']; clear_lift_subst.
+
+    admit.
+  - destruct xs.
+
+(λ, λ, var 0
+         ⋅ (F0 (var 2)
+            ⋅ ((lam_Y ⋅ F') ⋅ (λ, C ⋅ (λ, var 2 ⋅ (var 1 ⋅ var 0))))))
+
+
+    eapply steps_trans.
+    apply steps_beta.
+    cbn -[lam_Y F0 F']; clear_lift_subst.
+
+    eapply steps_trans.
+    apply steps_beta.
+    cbn -[lam_Y F0 F']; clear_lift_subst.
+
+
+    cbn.
+    eexists;split;[|apply steps_refl].
+    apply steps_app_left.
+    apply steps_beta.
+  unfold F_spec.
+Admitted.
+
+
+(* Lemma F_spec_proof C x xs:
+  closed0 C -> 
+  F_spec C x xs.
+Proof.
+  unfold F_spec.
+Admitted. *)
